src/proof/controllers/common.v
@@ -181,12 +181,12 @@ Definition owner_ref_key (owner_kind : go_string) (owner_meta : ObjectMetaV.t) :
 |}.
 
 Lemma wp_FilterPodsByOwner γ l owner owner_kind meta dq1
-    pods pod_dqs children_dq children_keys :
+    living_pods pod_dqs children_dq children_keys phase :
   {{{ is_pkg_init code.controllers.common.pkg_id.common ∗
       "#Hisk" ∷ is_kubernetes γ l ∗
       "#Hglobal_l" ∷ (global_addr apimodel.ModelState) ↦□ l ∗
       "Hdeepown_l_meta" ∷ ObjectMetaV.deepown_l owner meta dq1 ∗
-      "Hown_pod_meta_frags" ∷ ([∗ list] pod;pod_dq ∈ pods;pod_dqs,
+      "Hown_pod_meta_frags" ∷ ([∗ list] pod;pod_dq ∈ living_pods;pod_dqs,
         own_meta_frag γ (PodV.key pod)
           pod.(PodV.ObjectMeta').(ObjectMetaV.UID')
           pod_dq pod.(PodV.ObjectMeta')) ∗
@@ -195,31 +195,37 @@ Lemma wp_FilterPodsByOwner γ l owner owner_kind meta dq1
           meta.(ObjectMetaV.UID') children_dq children_keys ∗
       "Hown_terminating_children_frag" ∷
         own_terminating_children_frag γ (owner_ref_key owner_kind meta)
-          meta.(ObjectMetaV.UID') Quiescent ∗
-      "%Hnodup" ∷ ⌜ NoDup (PodV.key <$> pods) ⌝ ∗
-      "%Hdom_eq" ∷ ⌜ list_to_set (PodV.key <$> pods) = filter (λ key, key.(KKey.Kind') = "Pod"%go) children_keys ⌝ ∗
+          meta.(ObjectMetaV.UID') phase ∗
+      "%Hnodup" ∷ ⌜ NoDup (PodV.key <$> living_pods) ⌝ ∗
+      "%Hdom_eq" ∷ ⌜ list_to_set (PodV.key <$> living_pods) =
+        filter (λ key, key.(KKey.Kind') = "Pod"%go) children_keys ⌝ ∗
       "%Hslash_free" ∷ ⌜ slash_free owner_kind ∧
         slash_free meta.(ObjectMetaV.Namespace') ∧
         slash_free meta.(ObjectMetaV.Name') ∧
         slash_free meta.(ObjectMetaV.UID') ⌝
   }}}
     @! common.FilterPodsByOwner #owner #owner_kind
-  {{{ sl ptrs pods' dq', RET (#sl, #interface.nil);
+  {{{ sl ptrs all_pods dq', RET (#sl, #interface.nil);
       sl ↦* ptrs ∗
-      ([∗ list] ptr;pod ∈ ptrs;pods', PodV.deepown_l ptr pod dq') ∗
-      ⌜ ObjectMetaV.without_resource_version <$> (PodV.ObjectMeta' <$> pods') ≡ₚ
-        ObjectMetaV.without_resource_version <$> (PodV.ObjectMeta' <$> pods) ⌝ ∗
-      ⌜ Forall PodV.valid pods' ⌝ ∗
-      ⌜ NoDup (PodV.key <$> pods') ⌝ ∗
+      ([∗ list] ptr;pod ∈ ptrs;all_pods, PodV.deepown_l ptr pod dq') ∗
+      ⌜ ObjectMetaV.without_resource_version <$> (PodV.ObjectMeta' <$> filter is_pod_alive all_pods) ≡ₚ
+        ObjectMetaV.without_resource_version <$> (PodV.ObjectMeta' <$> living_pods) ⌝ ∗
+      ⌜ phase = Quiescent →
+        ObjectMetaV.without_resource_version <$> (PodV.ObjectMeta' <$> all_pods) ≡ₚ
+          ObjectMetaV.without_resource_version <$> (PodV.ObjectMeta' <$> living_pods) ⌝ ∗
+      ⌜ Forall PodV.valid all_pods ⌝ ∗
+      ⌜ NoDup (PodV.key <$> all_pods) ⌝ ∗
       ObjectMetaV.deepown_l owner meta dq1 ∗
-      ([∗ list] pod;pod_dq ∈ pods;pod_dqs,
+      ([∗ list] pod ∈ terminating_pods all_pods,
+        own_deletion_observed_frag γ (PodV.key pod) pod.(PodV.ObjectMeta').(ObjectMetaV.UID')) ∗
+      ([∗ list] pod;pod_dq ∈ living_pods;pod_dqs,
         own_meta_frag γ (PodV.key pod)
           pod.(PodV.ObjectMeta').(ObjectMetaV.UID')
           pod_dq pod.(PodV.ObjectMeta')) ∗
       own_children_frag γ (owner_ref_key owner_kind meta)
         meta.(ObjectMetaV.UID') children_dq children_keys ∗
       own_terminating_children_frag γ (owner_ref_key owner_kind meta)
-        meta.(ObjectMetaV.UID') Quiescent
+        meta.(ObjectMetaV.UID') phase
   }}}.
 Proof.
   wp_start as "H". iNamed "H". subst. wp_auto.
@@ -236,8 +242,8 @@ Proof.
   wp_apply (controller.wp_PodControllerIndexKey with "[$Howner_reference]").
   iIntros (index_key) "->". wp_auto.
   iNamedPrefix "Hdeepown_meta" "Htemp_".
-  wp_apply (wp_State__ByIndex_podController
-    _ _ _ _ pod_dqs _ _ _ children_dq
+  wp_apply (wp_State__ByIndex_podController_combined
+    _ _ _ _ pod_dqs _ _ _ children_dq phase
     with "[$Hown_pod_meta_frags $Hown_children_frag
       $Hown_terminating_children_frag]").
   { iFrame "#". iFrame "%". iPureIntro. rewrite Htemp_Hdeepown_namespace. rewrite Htemp_Hdeepown_name.
@@ -312,7 +318,7 @@ Proof.
       { rewrite <- (map_length interface.ok interfaces). rewrite Hsl_len1. word. }
       rewrite Hlen. apply take_ge. lia.
     }
-    iFrame "%".
+    iFrame "%". iFrame "Hindex_Hown_deletion_observed_frags".
 Qed.
 
 Lemma wp_FilterPodsByOwner_with_spec γ l owner owner_kind meta dq1
@@ -683,15 +689,16 @@ Proof.
     rewrite big_sepL2_replicate_r; [done|].
     iExact "Hown_pod_meta_frags". }
   iApply (wp_FilterPodsByOwner γ l owner owner_kind meta dq1
-    pods pod_dqs dq2 children_keys
+    pods pod_dqs dq2 children_keys Quiescent
     with "[-HΦ]").
   { iFrame "#". iFrame "%". iFrame. }
   iNext.
   iIntros (sl ptrs pods' dq') "H".
   iDestruct "H" as
-    "(Hsl & Hpods & %Hmeta_perm & %Hpods_valid & %Hpods_nodup &
-      Hdeepown_l_meta & Hown_pod_meta_frags & Hown_children_frag &
+    "(Hsl & Hpods & %Hliving_meta_perm & %Hmeta_perm & %Hpods_valid & %Hpods_nodup &
+      Hdeepown_l_meta & #Hown_deletion_observed_frags & Hown_pod_meta_frags & Hown_children_frag &
       Hown_terminating_children_frag)".
+  specialize (Hmeta_perm eq_refl).
   subst pod_dqs.
   iEval (rewrite big_sepL2_replicate_r; [done|])
     in "Hown_pod_meta_frags".
@@ -705,6 +712,84 @@ Proof.
   { rewrite own_meta_frag_list_as_erased_metas Hmeta_perm.
     iExact "Hown_pod_meta_frags". }
   iApply "HΦ". iFrame. iFrame "%".
+Qed.
+
+Lemma wp_FilterPodsByOwner_uniform_combined γ l owner owner_kind meta dq1 dq2
+    living_pods children_keys phase :
+  {{{ is_pkg_init code.controllers.common.pkg_id.common ∗
+      "#Hisk" ∷ is_kubernetes γ l ∗
+      "#Hglobal_l" ∷ (global_addr apimodel.ModelState) ↦□ l ∗
+      "Hdeepown_l_meta" ∷ ObjectMetaV.deepown_l owner meta dq1 ∗
+      "Hown_pod_meta_frags" ∷ ([∗ list] pod ∈ living_pods,
+        own_meta_frag γ (PodV.key pod)
+          pod.(PodV.ObjectMeta').(ObjectMetaV.UID') dq2 pod.(PodV.ObjectMeta')) ∗
+      "Hown_children_frag" ∷ own_children_frag γ (owner_ref_key owner_kind meta)
+        meta.(ObjectMetaV.UID') dq2 children_keys ∗
+      "Hown_terminating_children_frag" ∷
+        own_terminating_children_frag γ (owner_ref_key owner_kind meta)
+          meta.(ObjectMetaV.UID') phase ∗
+      "%Hnodup" ∷ ⌜ NoDup (PodV.key <$> living_pods) ⌝ ∗
+      "%Hdom_eq" ∷ ⌜ list_to_set (PodV.key <$> living_pods) =
+        filter (λ key, key.(KKey.Kind') = "Pod"%go) children_keys ⌝ ∗
+      "%Hslash_free" ∷ ⌜ slash_free owner_kind ∧
+        slash_free meta.(ObjectMetaV.Namespace') ∧
+        slash_free meta.(ObjectMetaV.Name') ∧
+        slash_free meta.(ObjectMetaV.UID') ⌝
+  }}}
+    @! common.FilterPodsByOwner #owner #owner_kind
+  {{{ sl ptrs all_pods dq', RET (#sl, #interface.nil);
+      sl ↦* ptrs ∗
+      ([∗ list] ptr;pod ∈ ptrs;all_pods, PodV.deepown_l ptr pod dq') ∗
+      ⌜ ObjectMetaV.without_resource_version <$> (PodV.ObjectMeta' <$> filter is_pod_alive all_pods) ≡ₚ
+        ObjectMetaV.without_resource_version <$> (PodV.ObjectMeta' <$> living_pods) ⌝ ∗
+      ⌜ Forall PodV.valid all_pods ⌝ ∗
+      ⌜ NoDup (PodV.key <$> all_pods) ⌝ ∗
+      ObjectMetaV.deepown_l owner meta dq1 ∗
+      ([∗ list] pod ∈ terminating_pods all_pods,
+        own_deletion_observed_frag γ (PodV.key pod) pod.(PodV.ObjectMeta').(ObjectMetaV.UID')) ∗
+      ([∗ list] pod ∈ filter is_pod_alive all_pods,
+        own_meta_frag γ (PodV.key pod)
+          pod.(PodV.ObjectMeta').(ObjectMetaV.UID') dq2 pod.(PodV.ObjectMeta')) ∗
+      own_children_frag γ (owner_ref_key owner_kind meta)
+        meta.(ObjectMetaV.UID') dq2 children_keys ∗
+      own_terminating_children_frag γ (owner_ref_key owner_kind meta)
+        meta.(ObjectMetaV.UID') phase
+  }}}.
+Proof.
+  iIntros (Φ) "H HΦ".
+  iDestruct "H" as
+    "(#Hinit & #Hisk & #Hglobal_l & Hdeepown_l_meta &
+      Hown_pod_meta_frags & Hown_children_frag & Hown_terminating_children_frag &
+      %Hnodup & %Hdom_eq & %Hslash_free)".
+  set pod_dqs := replicate (length living_pods) dq2.
+  iAssert (([∗ list] pod;pod_dq ∈ living_pods;pod_dqs,
+      own_meta_frag γ (PodV.key pod) pod.(PodV.ObjectMeta').(ObjectMetaV.UID')
+        pod_dq pod.(PodV.ObjectMeta')))%I
+    with "[Hown_pod_meta_frags]" as "Hown_pod_meta_frags".
+  { subst pod_dqs. rewrite big_sepL2_replicate_r; [done|].
+    iExact "Hown_pod_meta_frags". }
+  iApply (wp_FilterPodsByOwner γ l owner owner_kind meta dq1
+    living_pods pod_dqs dq2 children_keys phase with "[-HΦ]").
+  { iFrame "#". iFrame "%". iFrame. }
+  iNext.
+  iIntros (sl ptrs all_pods dq') "H".
+  iDestruct "H" as
+    "(Hsl & Hpods & %Hliving_meta_perm & %Hquiescent_meta_perm &
+      %Hpods_valid & %Hpods_nodup & Hdeepown_l_meta & #Hown_deletion_observed_frags &
+      Hown_pod_meta_frags & Hown_children_frag & Hown_terminating_children_frag)".
+  subst pod_dqs.
+  iEval (rewrite big_sepL2_replicate_r; [done|]) in "Hown_pod_meta_frags".
+  iEval (rewrite own_meta_frag_list_as_erased_metas) in "Hown_pod_meta_frags".
+  iAssert (([∗ list] pod ∈ filter is_pod_alive all_pods,
+      own_meta_frag γ (PodV.key pod) pod.(PodV.ObjectMeta').(ObjectMetaV.UID')
+        dq2 pod.(PodV.ObjectMeta')))%I
+    with "[Hown_pod_meta_frags]" as "Hown_living_pod_meta_frags".
+  { rewrite own_meta_frag_list_as_erased_metas Hliving_meta_perm.
+    iExact "Hown_pod_meta_frags". }
+  iApply "HΦ".
+  iFrame "Hsl Hpods Hdeepown_l_meta Hown_deletion_observed_frags
+    Hown_living_pod_meta_frags Hown_children_frag Hown_terminating_children_frag".
+  iFrame "%".
 Qed.
 
 End proof.
